feat: prove that omega-regularity is closed under union and is universe-polymorphic (#168)
This patch proves that:
(1) omega-regular languages are closed under finite union, and
(2) the definition of omega-regular languages is universe-polymorphic.
The `iSum` construction used to prove (1) actually works over an
arbitrary indexed family of NA.Buchi automata.

---------

Co-authored-by: Chris Henson <chrishenson.net@gmail.com>

Cslib/Computability/Languages/OmegaRegularLanguage.lean
@@ -5,8 +5,11 @@ Authors: Ching-Tsun Chou
 -/
 
 import Cslib.Computability.Automata.DABuchi
+import Cslib.Computability.Automata.NABuchiEquiv
+import Cslib.Computability.Automata.Sum
 import Cslib.Computability.Languages.ExampleEventuallyZero
 import Cslib.Computability.Languages.RegularLanguage
+import Mathlib.Data.Finite.Sigma
 
 /-!
 # ω-Regular languages
@@ -17,14 +20,31 @@ This file defines ω-regular languages and proves some properties of them.
 open Set Function Filter Cslib.ωSequence Cslib.Automata ωAcceptor
 open scoped Computability
 
+universe u v
+
 namespace Cslib.ωLanguage
 
-variable {Symbol : Type*}
+variable {Symbol : Type u}
 
 /-- An ω-language is ω-regular iff it is accepted by a
 finite-state nondeterministic Buchi automaton. -/
 def IsRegular (p : ωLanguage Symbol) :=
-  ∃ State : Type, ∃ _ : Finite State, ∃ na : NA.Buchi State Symbol, language na = p
+  ∃ (State : Type) (_ : Finite State) (na : NA.Buchi State Symbol), language na = p
+
+/-- Helper lemma for `isRegular_iff` below. -/
+private lemma isRegular_iff.helper.{v'} {Symbol : Type u} {p : ωLanguage Symbol}
+    (h : ∃ (σ : Type v) (_ : Finite σ) (na : NA.Buchi σ Symbol), language na = p) :
+    ∃ (σ' : Type v') (_ : Finite σ') (na : NA.Buchi σ' Symbol), language na = p := by
+  have ⟨σ, _, na, h_na⟩ := h
+  have ⟨σ', ⟨f⟩⟩ := Small.equiv_small.{v', v} (α := σ)
+  use σ', Finite.of_equiv σ f, na.reindex f
+  rwa [NA.Buchi.reindex_language_eq]
+
+/-- The state space of the accepting finite-state nondeterministic Buchi automaton
+can in fact be universe-polymorphic. -/
+theorem isRegular_iff {p : ωLanguage Symbol} :
+    p.IsRegular ↔ ∃ (σ : Type v) (_ : Finite σ) (na : NA.Buchi σ Symbol), language na = p :=
+  ⟨isRegular_iff.helper, isRegular_iff.helper⟩
 
 /-- The ω-language accepted by a finite-state deterministic Buchi automaton is ω-regular. -/
 theorem IsRegular.of_da_buchi {State : Type} [Finite State] (da : DA.Buchi State Symbol) :
@@ -34,8 +54,8 @@ theorem IsRegular.of_da_buchi {State : Type} [Finite State] (da : DA.Buchi State
 /-- There is an ω-regular language that is not accepted by any deterministic Buchi automaton,
 where the automaton is not even required to be finite-state. -/
 theorem IsRegular.not_da_buchi :
-  ∃ Symbol : Type, ∃ p : ωLanguage Symbol, p.IsRegular ∧
-    ¬ ∃ State : Type, ∃ da : DA.Buchi State Symbol, language da = p := by
+  ∃ (Symbol : Type) (p : ωLanguage Symbol), p.IsRegular ∧
+    ¬ ∃ (State : Type) (da : DA.Buchi State Symbol), language da = p := by
   refine ⟨Fin 2, Example.eventually_zero, ?_, ?_⟩
   · use Fin 2, inferInstance, Example.eventually_zero_na,
       Example.eventually_zero_accepted_by_na_buchi
@@ -44,14 +64,59 @@ theorem IsRegular.not_da_buchi :
     grind [DA.buchi_eq_finAcc_omegaLim]
 
 /-- The ω-limit of a regular language is ω-regular. -/
+@[simp]
 theorem IsRegular.regular_omegaLim {l : Language Symbol}
     (h : l.IsRegular) : (l↗ω).IsRegular := by
   obtain ⟨State, _, ⟨da, acc⟩, rfl⟩ := Language.IsRegular.iff_cslib_dfa.mp h
   grind [IsRegular.of_da_buchi, =_ DA.buchi_eq_finAcc_omegaLim]
 
+/-- The empty language is ω-regular. -/
+@[simp]
+theorem IsRegular.bot : (⊥ : ωLanguage Symbol).IsRegular := by
+  let na : NA.Buchi Unit Symbol := {
+    Tr _ _ _ := False
+    start := ∅
+    accept := ∅ }
+  use Unit, inferInstance, na
+  ext xs
+  simp [na]
+
+/-- The union of two ω-regular languages is ω-regular. -/
+@[simp]
+theorem IsRegular.sup {p1 p2 : ωLanguage Symbol}
+    (h1 : p1.IsRegular) (h2 : p2.IsRegular) : (p1 ⊔ p2).IsRegular := by
+  obtain ⟨State1, h_fin1, ⟨na1, acc1⟩, rfl⟩ := h1
+  obtain ⟨State2, h_fin1, ⟨na2, acc2⟩, rfl⟩ := h2
+  let State : Fin 2 → Type
+    | 0 => State1 | 1 => State2
+  let na : (i : Fin 2) → NA (State i) Symbol
+    | 0 => na1 | 1 => na2
+  let acc : (i : Fin 2) → Set (State i)
+    | 0 => acc1 | 1 => acc2
+  have : ∀ i, Finite (State i) := by grind
+  use (Σ i : Fin 2, State i), inferInstance, ⟨(NA.iSum na), (⋃ i, Sigma.mk i '' (acc i))⟩
+  ext xs
+  simp only [NA.Buchi.iSum_language_eq, mem_sup, mem_language]
+  rw [mem_iUnion, Fin.exists_fin_two]
+  grind
+
+/-- The union of any finite number of ω-regular languages is ω-regular. -/
+@[simp]
+theorem IsRegular.iSup {I : Type*} [Finite I] {s : Set I} {p : I → ωLanguage Symbol}
+    (h : ∀ i ∈ s, (p i).IsRegular) : (⨆ i ∈ s, p i).IsRegular := by
+  generalize h_n : s.ncard = n
+  induction n generalizing s
+  case zero =>
+    have := ncard_eq_zero (s := s)
+    grind [IsRegular.bot, iSup_bot]
+  case succ n h_ind =>
+    obtain ⟨i, t, h_i, rfl, rfl⟩ := (ncard_eq_succ (s := s)).mp h_n
+    rw [iSup_insert]
+    grind [IsRegular.sup]
+
 /-- McNaughton's Theorem. -/
 proof_wanted IsRegular.iff_da_muller {p : ωLanguage Symbol} :
     p.IsRegular ↔
-    ∃ State : Type, ∃ _ : Finite State, ∃ da : DA.Muller State Symbol, language da = p
+    ∃ (State : Type) (_ : Finite State) (da : DA.Muller State Symbol), language da = p
 
 end Cslib.ωLanguage
