Cslib/Computability/Automata/DAToNA.lean
@@ -26,14 +26,14 @@ def toNA (a : DA State Symbol) : NA State Symbol :=
 instance : Coe (DA State Symbol) (NA State Symbol) where
   coe := toNA
 
-open scoped FLTS NA in
+open scoped FLTS NA NA.Run in
 @[simp, scoped grind =]
 theorem toNA_run {a : DA State Symbol} {xs : ωSequence Symbol} {ss : ωSequence State} :
     a.toNA.Run xs ss ↔ a.run xs = ss := by
   constructor
   · rintro _
     ext n
-    induction n <;> grind
+    induction n <;> grind [NA.Run]
   · grind
 
 namespace FinAcc
