Cslib/Computability/Automata/NA.lean
@@ -1,7 +1,7 @@
 /-
 Copyright (c) 2025 Fabrizio Montesi. All rights reserved.
 Released under Apache 2.0 license as described in the file LICENSE.
-Authors: Fabrizio Montesi, Ching-Tsun Chou
+Authors: Fabrizio Montesi, Ching-Tsun Chou, Chris Henson.
 -/
 
 import Cslib.Computability.Automata.Acceptor
@@ -40,9 +40,27 @@ namespace NA
 variable {State : Type _} {Symbol : Type _}
 
 /-- Infinite run. -/
-@[scoped grind =]
 def Run (na : NA State Symbol) (xs : ωSequence Symbol) (ss : ωSequence State) :=
   ss 0 ∈ na.start ∧ ∀ n, na.Tr (ss n) (xs n) (ss (n + 1))
+
+-- The following lemmas help `grind` deal with the definition of `NA.Run` better.
+section NARunGrind
+
+variable {na : NA State Symbol} {xs : ωSequence Symbol} {ss : ωSequence State}
+
+@[scoped grind <=]
+lemma Run.mk (h₁ : ss 0 ∈ na.start) (h₂ : ∀ n, na.Tr (ss n) (xs n) (ss (n + 1))) : Run na xs ss
+  := ⟨h₁, h₂⟩
+
+@[scoped grind →]
+lemma Run.start (run : Run na xs ss) : ss 0 ∈ na.start :=
+  run.left
+
+@[scoped grind =>]
+lemma Run.trans (run : Run na xs ss) : ∀ n, na.Tr (ss n) (xs n) (ss (n + 1)) :=
+  run.right
+
+end NARunGrind
 
 /-- A nondeterministic automaton that accepts finite strings (lists of symbols). -/
 structure FinAcc (State Symbol : Type*) extends NA State Symbol where
