Cslib/Computability/Automata/Sum.lean
@@ -1,0 +1,74 @@
+/-
+Copyright (c) 2025 Ching-Tsun Chou. All rights reserved.
+Relexsed under Apache 2.0 license xs described in the file LICENSE.
+Authors: Ching-Tsun Chou
+-/
+
+import Cslib.Computability.Automata.NA
+
+/-! # Sum of automata. -/
+
+open Set Function Filter Cslib.ωSequence
+open scoped Cslib.LTS
+
+namespace Cslib.Automata.NA
+open scoped Run
+
+variable {Symbol I : Type*} {State : I → Type*}
+
+@[scoped grind =]
+def iSum (na : (i : I) → NA (State i) Symbol) : NA (Σ i, State i) Symbol where
+  start := ⋃ i, Sigma.mk i '' (na i).start
+  Tr s x t := ∃ i s_i t_i, (na i).Tr s_i x t_i ∧ ⟨i, s_i⟩ = s ∧ ⟨i, t_i⟩ = t
+
+@[simp, scoped grind =]
+theorem iSum_run_iff {na : (i : I) → NA (State i) Symbol}
+    {xs : ωSequence Symbol} {ss : ωSequence (Σ i, State i)} :
+    (iSum na).Run xs ss ↔ ∃ i ss_i, (na i).Run xs ss_i ∧ ss_i.map (Sigma.mk i) = ss := by
+  constructor
+  · rintro ⟨h_init, h_next⟩
+    obtain ⟨i, s0, h_s0, h_ss0⟩ := mem_iUnion.mp h_init
+    have h_exists n : ∃ s_i, ⟨i, s_i⟩ = ss n := by
+      induction n
+      case zero => use s0
+      case succ n h_ind =>
+        obtain ⟨j, s_j, t_j, _⟩ := h_next n
+        grind
+    choose ss_i h_ss_i using h_exists
+    use i, ss_i
+    refine ⟨⟨?_, ?_⟩, ?_⟩
+    · grind
+    · intro n
+      obtain ⟨j, _⟩ := h_next n
+      grind
+    · ext <;> grind
+  · rintro ⟨i, ss, h_run, rfl⟩
+    constructor
+    · simp only [iSum, get_map, mem_iUnion, mem_image, Sigma.mk.injEq]
+      grind
+    · intro n
+      use i
+      grind [Run]
+
+namespace Buchi
+
+open ωAcceptor
+
+@[simp]
+theorem iSum_language_eq {na : (i : I) → NA (State i) Symbol} {acc : (i : I) → Set (State i)} :
+    language (Buchi.mk (iSum na) (⋃ i, Sigma.mk i '' (acc i))) =
+    ⋃ i, language (Buchi.mk (na i) (acc i)) := by
+  ext xs
+  rw [mem_iUnion]
+  constructor
+  · rintro ⟨ss, h_run, h_acc⟩
+    simp only [mem_iUnion] at h_acc
+    grind
+  · rintro ⟨i, ss_i, _⟩
+    use ss_i.map (Sigma.mk i)
+    simp only [mem_iUnion]
+    grind
+
+end Buchi
+
+end Cslib.Automata.NA
